src/demo/flasher/NotAutomat.thy
@@ -17,26 +17,36 @@ abbreviation notStep::"(S_not \<Rightarrow> (inNot\<^sup>\<Omega> \<rightarrow> 
 "notStep \<equiv> dawStateSem not_smap.da"
 
 definition notSpf::"(inNot\<^sup>\<Omega> \<rightarrow> outNot\<^sup>\<Omega>)"where
-"notSpf = dawSem not_smap.da"
+"notSpf = dasSem (dAutomaton_weak.extend not_smap.da (dAutomaton_strong.fields (notOutSBE.setter True)))"
+
+
+lemma dasinitout_well:"(dasInitOut
+         (dAutomaton_weak.extend daw
+           (dAutomaton_strong.fields
+             sbe))) = sbe" (*How proof this?*)
+  sorry
+
+lemma das2daw_trunc_well:"dAutomaton_weak.truncate
+                (dAutomaton_weak.extend da
+                  (dAutomaton_strong.fields sbe)) = da" (*How proof this?*)
+  sorry
 
 lemma notingetset_eq:"notInSBE.getterSB\<cdot>(notInSBE.setterSB\<cdot>s) = s"
-  by(simp add: notInSBE.getset_eq)
+  by(simp)
 
 lemma notoutgetset_eq:"notOutSBE.getterSB\<cdot> (notOutSBE.setterSB\<cdot>s) = s"
-  by(simp add: notOutSBE.getset_eq)
-(*
+  by(simp)
+
 lemma notstep2smap:"notOutSBE.getterSB\<cdot>(notStep state\<cdot>(notInSBE.setterSB\<cdot>input)) = (smap not_smap.smapTransition)\<cdot>input"
-  by (simp add: notInSBE.getset_eq not_smap.daut2smap notoutgetset_eq)
+  by (metis (full_types) S_not.exhaust not_smap.daut2smap)
 
 thm dAutomaton_weak.select_convs
 
-lemma "notOutSBE.getterSB\<cdot>(notSpf\<cdot>(notInSBE.setterSB\<cdot>input)) = \<up>True \<bullet>(smap not_smap.smapTransition)\<cdot>input"
-  apply(simp add: notSpf_def dasSem_def)
-  apply(subst notOutSBE.gettersb_unfold)
-  apply(simp add: dAnot_def)
-  by (metis dAnot_def dAutomaton_weak.select_convs(1) notstep2smap)
 
-lemma "smap not_smap.smapTransition\<cdot>(\<up>bool \<bullet> s) = \<up>(\<not>bool) \<bullet> smap not_smap.smapTransition\<cdot>s"
-  by(simp add: dAnot_def dNot_transition_def)
-*)
+lemma "notOutSBE.getterSB\<cdot>(notSpf\<cdot>(notInSBE.setterSB\<cdot>input)) = \<up>True \<bullet>(smap not_smap.smapTransition)\<cdot>input"
+  by(simp add: notSpf_def dasSem_def dasinitout_well das2daw_trunc_well dawSem_def notstep2smap)
+
+lemma not_step:"smap not_smap.smapTransition\<cdot>(\<up>bool \<bullet> s) = \<up>(\<not>bool) \<bullet> smap not_smap.smapTransition\<cdot>s"
+  by simp
+
 end
